Fix up one lemma on the Poly side. Lib.Unlib to be able to state the signature of EverCrypt.Poly1305. Attempted to use Chris' lemma -- still needs work to derive the proper post-condition

providers/evercrypt/fst/EverCrypt.Poly1305.fst
@@ -6,11 +6,15 @@ module B = LowStar.Buffer
 module U32 = FStar.UInt32
 module ST = FStar.HyperStack.ST
 module F = Hacl.Impl.Poly1305.Fields
+module S = FStar.Seq
 
 open FStar.HyperStack.ST
 
 #reset-options "--max_fuel 0 --max_ifuel 0"
 
+friend Lib.IntTypes
+
+#push-options "--z3rlimit 200"
 let poly1305 dst src len key =
   let h0 = ST.get () in
   let avx2 = EverCrypt.AutoConfig2.has_avx2 () in
@@ -23,15 +27,34 @@ let poly1305 dst src len key =
     Hacl.Spec.Poly1305.Vec.poly1305_vec_is_poly1305 #2 (B.as_seq h0 src) (B.as_seq h0 key)
   end else if EverCrypt.TargetConfig.x64 then begin
     push_frame ();
+    // Vale wants a large context
     let ctx = B.alloca 0uy 192ul in
-    B.blit key 0ul ctx 16ul 64ul;
-    Poly_stdcalls.poly1305 ctx src (FStar.Int.Cast.Full.uint32_to_uint64 len);
-    B.blit ctx 0ul dst 0ul 16ul;
+    // With the key located at bytes [ 24; 56 )
+    B.blit key 0ul ctx 24ul 32ul;
+    // With an extra constraint on the size of the input buffer (to be alleviated)
+    assume (U32.v len % 16 = 0);
+
+    // Call Vale
     let h1 = ST.get () in
-    X64.Poly1305.CallingFromLowStar.lemma_call_poly1305 h0 h1 ctx (*inp*)src (Arch.BufferFriend.to_bytes (B.as_seq h0 src)) (Arch.BufferFriend.to_bytes (B.as_seq h0 key));
-    Poly1305.Equiv.lemma_poly1305_equiv (Arch.BufferFriend.to_bytes (B.as_seq h0 src)) (Arch.BufferFriend.to_bytes (B.as_seq h0 key));
-    assert (B.as_seq h1 dst == Spec.Poly1305.poly1305 (B.as_seq h0 src) (B.as_seq h0 key));
-    pop_frame ()
+    Poly_stdcalls.poly1305 ctx src (FStar.Int.Cast.Full.uint32_to_uint64 len);
+    let h2 = ST.get () in
+
+    X64.Poly1305.CallingFromLowStar.lemma_call_poly1305 h1 h2 ctx (*inp*)src
+      (Arch.BufferFriend.to_bytes (B.as_seq h1 src))
+      (Arch.BufferFriend.to_bytes (B.as_seq h1 key));
+
+    Poly1305.Equiv.lemma_poly1305_equiv (Arch.BufferFriend.to_bytes (B.as_seq h1 src))
+      (Arch.BufferFriend.to_bytes (B.as_seq h1 key));
+
+    assume (S.slice (B.as_seq h2 ctx) 0 16 `S.equal`
+      Spec.Poly1305.poly1305 (B.as_seq h1 src) (B.as_seq h1 key));
+
+    B.blit ctx 0ul dst 0ul 16ul;
+    pop_frame ();
+
+    let h3 = ST.get () in
+    assert (B.as_seq h3 dst `S.equal` Spec.Poly1305.poly1305 (B.as_seq h0 src) (B.as_seq h0 key))
+
   end else begin
     Hacl.Poly1305_32.poly1305_mac dst src len key;
     Hacl.Spec.Poly1305.Vec.poly1305_vec_is_poly1305 #1 (B.as_seq h0 src) (B.as_seq h0 key)
