lib/Lib.Unlib.fst
@@ -1,0 +1,5 @@
+module Lib.Unlib
+
+friend Lib.IntTypes
+
+let reveal_secret8 () = ()
