providers/evercrypt/EverCrypt.Poly1305.fsti
@@ -11,11 +11,12 @@ open FStar.HyperStack.ST
 val poly1305: dst:B.buffer UInt8.t { B.length dst = 16 } ->
   src:B.buffer UInt8.t ->
   len:U32.t { U32.v len = B.length src } ->
-  key:B.buffer UInt8.t { B.length dst = 32 } ->
+  key:B.buffer UInt8.t { B.length key = 32 } ->
   Stack unit
     (requires fun h ->
       B.live h src /\ B.live h dst /\ B.live h key /\
       B.disjoint dst src /\ B.disjoint dst key)
     (ensures fun h0 _ h1 ->
-      B.(modifies (loc_buffer dst) h0 h1 /\
-      B.as_seq h1 dst == Spec.Poly1305.poly1305 (B.as_seq h0 src) (B.as_seq h0 key)))
+      B.(modifies (loc_buffer dst) h0 h1 /\ (
+      Lib.Unlib.reveal_secret8 ();
+      B.as_seq h1 dst == Spec.Poly1305.poly1305 (B.as_seq h0 src) (B.as_seq h0 key))))
